Verified SqrtUpperBound function

basic_arithmetic.dfy
@@ -9,97 +9,40 @@ module BasicArithmetic {
   }
 
   /** Positive square root (abstract). */
-  ghost opaque function {:axiom} Sqrt(x: real): (r: real)
+  ghost opaque function Sqrt(x: real): (r: real)
     requires x >= 0.0
-    ensures r >= 0.0
-    ensures r * r == x
+    ensures {:axiom} r >= 0.0
+    ensures {:axiom} r * r == x
 
-  /** Positive 2^i'th root (abstract). */
-  ghost function Power2Root(x: real, i: nat): (r: real)
-    requires x >= 0.0
+  /** The square root of 0 is 0. */
+  lemma SqrtZeroIsZero()
+    ensures Sqrt(0.0) == 0.0
   {
-    if i == 0 then x else Sqrt(Power2Root(x, i - 1))
-  }
-
-  /** Computes an upper bound on the positive square root of x. */
-  method SqrtUpperBound(a: real) returns (r: real)
-    requires a >= 0.0
-    ensures r >= Sqrt(a)
-  {
-    r := 0.5 * (a + 1.0);
-    var i := 1;
-    while i < 10 // fixme: we'd like to stop when r * r <= a + e for some e
-      invariant r >= Sqrt(a) && r > 0.0
-    {
-      assert Square((r - Sqrt(a))) >= 0.0;
-      r := 0.5 * (r + a / r);
-      i := i + 1;
+    if Sqrt(0.0) != 0.0 {
+      calc {
+        0.0;
+        < Sqrt(0.0) * Sqrt(0.0);
+        == 0.0;
+      }
     }
   }
 
-  /** Computes an upper bound on the positive square root of x. */
-  method Power2RootUpperBound(x: real, i: nat) returns (r: real)
-    requires x >= 0.0
-    ensures r >= Power2Root(x, i)
-  {
-    r := 1.0;
-    assume r >= Power2Root(x, i); // todo
-  }
-
-  lemma Power2RootDef(x: real, i: nat)
-    requires x >= 0.0
-    ensures Power2Root(x, i + 1) == Power2Root(Sqrt(x), i)
-  {}
-
-  lemma Power2RootMonotonic(x: real, y: real, i: nat)
-    requires 0.0 <= x <= y
-    ensures Power2Root(x, i) <= Power2Root(y, i)
-  {
-    if i != 0 {
-      Power2RootMonotonic(x, y, i - 1);
-      MonotonicSqrt(Power2Root(x, i - 1), Power2Root(y, i - 1));
-    }
-  }
-
-  /** Absolute value of the given number. */
-  ghost function Abs(x: real): real
-  {
-    if x >= 0.0 then x else -x
-  }
-
-  /** Square of the given number. */
-  function Square(x: real): (r: real)
-    ensures r >= 0.0
-  {
-    x * x
-  }
-
-  /** 
-   * The Sqrt function used in this file returns the positive square root.
-   * Therefore, Sqrt(x^2) == |x|.
-   */
-  lemma SqrtOfSquare()
-    ensures forall x: real :: Sqrt(Square(x)) == Abs(x)
-  {
-    assert forall x: real ::
-      Sqrt(Square(x)) * Sqrt(Square(x)) == Abs(x) * Abs(x);
-    forall x: real {
-      PositiveSquaresEquality(Sqrt(Square(x)), Abs(x));
-    }
-  }
-
-  /** For non-negative reals x and y, if x^2 == y^2 then x == y. */
-  lemma PositiveSquaresEquality(x: real, y: real)
-    requires x >= 0.0 && y >= 0.0
-    requires x * x == y * y
-    ensures x == y
+  /** For reals x and y where 0 <= y, if x^2 <= y^2 then x <= y. */
+  lemma MonotonicSqrt(x: real, y: real)
+    requires 0.0 <= y
+    requires x * x <= y * y
+    ensures x <= y
   {
     if x > y {
-      IncreaseSquare(x, y);
-    } else if x < y {
-      IncreaseSquare(y, x);
+      if y == 0.0 {
+        Increase(x, 0.0, x);
+      } else {
+        Increase(x, y, x);
+        Increase(x, y, y);
+      }
+      assert false;
     }
-  } 
+  }
 
   /** For reals x and y, and some real z > 0, if x > y then x * z > y * z. */
   lemma Increase(x: real, y: real, z: real)
@@ -108,85 +51,107 @@ module BasicArithmetic {
     ensures x * z > y * z
   {}
 
-  /** For any real number x, if x * x == 0 then x == 0. */
-  lemma Zero(x: real)
-    requires x * x == 0.0
-    ensures x == 0.0
-  {
-    // Assume the conclusion is false
-    if x != 0.0 {
-      // Case 1: x > 0
-      if x > 0.0 {
-        // Then x * x > x * 0
-        Increase(x, 0.0, x);
-        // This violates the requires clause
-        assert false;
-      // Case 2: x < 0
-      } else if x < 0.0 {
-        // Then -x * -x > -x * 0
-        Increase(-x, 0.0, -x);
-        // This violates the requires clause
-        assert false;
-      }
-    }
-  }
-
-  /** For non-negative reals x and y, if y < x then y^2 < x^2. */
-  lemma IncreaseSquare(x: real, y: real)
-    requires 0.0 <= y < x
-    ensures y * y < x * x
-  {
-    if y == 0.0 {
-      // x * x > x * 0
-      Increase(x, 0.0, x);
-      // Since x * 0 == 0 == y * y, we have x * x > y * y
-    } else {
-      // x * x > x * y
-      Increase(x, y, x);
-      // x * y > y * y
-      Increase(x, y, y);
-      // Thus x * x > y * y by transitivity of '>'
-    }
-  }
-
-  /** For non-negative reals x and y, if x <= y then sqrt(x) <= sqrt(y). */
-  lemma MonotonicSqrt(x: real, y: real)
-    requires 0.0 <= x <= y
-    ensures Sqrt(x) <= Sqrt(y)
-  {
-    if Sqrt(x) > Sqrt(y) {
-      // Then sqrt(x) * sqrt(x) > sqrt(y) * sqrt(y)
-      IncreaseSquare(Sqrt(x), Sqrt(y));
-      // Hence x > y, which is a contradiction
-      assert false;
-    }
-  }
-
-  /** For any non-negative reals x and y, x^2 <= y^2. */
-  lemma MonotonicSquarePositive(x: real, y: real)
-    requires 0.0 <= x <= y
-    ensures Square(x) <= Square(y)
-  {
-    assert 0.0 <= y;
-  }
-
-  /** For any real number x, we have |x|^2 == x^2. */
-  lemma AbsoluteSquare(x: real)
-    ensures Square(Abs(x)) == Square(x)
+  lemma SmallerDenominator(x: real, y: real, z: real)
+    requires 0.0 <= x
+    requires 0.0 < y <= z
+    ensures x / z <= x / y
   {}
 
-  /** For any real numbers x and y, if |x| <= |y| then x^2 <= y^2. */
-  lemma MonotonicSquare(x: real, y: real)
-    requires Abs(x) <= Abs(y)
-    ensures Square(x) <= Square(y)
+  lemma PositiveSquare(x: real)
+    ensures 0.0 <= x * x
+  {}
+
+  // ===========================================================================
+
+  method SqrtUpperBound(x: real, e: real) returns (r: real)
+    requires x >= 0.0
+    requires e > 0.0
+    ensures Sqrt(x) <= r <= Sqrt(x) + e
   {
-    // |x| <= |y|
-    MonotonicSquarePositive(Abs(x), Abs(y));
-    // 1: |x|^2 <= |y|^2
-    AbsoluteSquare(x);
-    // 2: |x|^2 == x^2
-    AbsoluteSquare(y);
-    // 3: |y|^2 == y^2
-    // From 1, 2, 3: x^2 <= y^2
+    if x == 0.0 {
+      SqrtZeroIsZero();
+      return 0.0;
+    }
+    r := if x < 1.0 then 1.0 else x;
+    while r >= e && (r - e) * (r - e) > x
+      invariant 0.0 < Sqrt(x) <= r
+      decreases 2.0 / e * r
+    {
+      ghost var R := r;
+
+      // lower bounds on R
+      assert R >= Sqrt(x) + e by {
+        assert (r - e) * (r - e) > x;
+        PositiveSquare(r - e);
+        MonotonicSqrt(Sqrt(x), r - e);
+        assert r - e >= Sqrt(x);
+        assert R >= Sqrt(x) + e;
+      }
+
+      // maintain upper bound
+      assert Sqrt(x) <= 0.5 * (r + x / r) by {
+        PositiveSquare(r - Sqrt(x));
+        assert 0.0 <= (r - Sqrt(x)) * (r - Sqrt(x)); // 0.0 <= any square
+        assert 0.0 <= r * r - 2.0 * r * Sqrt(x) + x; // distribute
+        assert 0.0 <= (r * r - 2.0 * r * Sqrt(x) + x) / r; // divide by r
+        assert 0.0 <=  r     - 2.0 * Sqrt(x)     + x / r; // simplify
+        assert 2.0 * Sqrt(x) <= r + x / r; // rearrange
+        assert Sqrt(x) <= 0.5 * (r + x / r); // divide by 2
+      }
+      
+      // update r
+      r := 0.5 * (r + x / r);
+      assert Sqrt(x) <= r;
+      
+      // termination
+      assert 2.0 / e * R - 2.0 / e * r >= 1.0 by {
+        calc {
+          R - r;
+          ==
+          calc {
+            r;
+            ==
+            0.5 * (R + x / R);
+            ==
+            (R + x / R) / 2.0;
+          }
+          R - (R + x / R) / 2.0;
+          >=
+          calc {
+            R + x / R;
+            <=
+            calc {
+              R;
+              >=
+              Sqrt(x);
+            }
+            {
+              SmallerDenominator(x, Sqrt(x), R);
+            }
+            R + x / Sqrt(x);
+          }
+          R - (R + x / Sqrt(x)) / 2.0;
+          ==
+          R - (R + Sqrt(x)) / 2.0;
+          ==
+          (R - Sqrt(x)) / 2.0;
+          >=
+          (Sqrt(x) + e - Sqrt(x)) / 2.0;
+          ==
+          e / 2.0;
+        }
+        assert R - r >= e / 2.0;
+        assert 2.0 * R - 2.0 * r >= e;
+        assert (1.0 / e) * 2.0 * R - (1.0 / e) * 2.0 * r >= (1.0 / e) * e;
+        assert 2.0 / e * R - 2.0 / e * r >= 1.0;
+      }
+    }
+    assert r < e || (r - e) * (r - e) <= x;
+    if (r >= e) {
+      PositiveSquare(r - e);
+      MonotonicSqrt(r - e, Sqrt(x));
+    }
+    assert r - e <= Sqrt(x);
+    assert r <= Sqrt(x) + e;
   }
 }
